securedrop-protocol/protocol-minimal/proofs/fstar/models/Libcrux_ecdh.Hacl.Curve25519.fsti
@@ -1,0 +1,6 @@
+module Libcrux_ecdh.Hacl.Curve25519
+#set-options "--fuel 0 --ifuel 1 --z3rlimit 15"
+open FStar.Mul
+open Core_models
+
+type t_Error = | Error_InvalidInput : t_Error
