securedrop-protocol/protocol-minimal/proofs/fstar/models/Libcrux_ecdh.Hacl.fsti
@@ -1,0 +1,9 @@
+module Libcrux_ecdh.Hacl
+#set-options "--fuel 0 --ifuel 1 --z3rlimit 15"
+open FStar.Mul
+open Core_models
+
+/// Unified error type.
+type t_Error =
+  | Error_Curve25519 : Libcrux_ecdh.Hacl.Curve25519.t_Error -> t_Error
+  | Error_P256 : Libcrux_ecdh.Hacl.P256.t_Error -> t_Error
