securedrop-protocol/protocol-minimal/proofs/fstar/models/Libcrux_ecdh.P256_internal.fsti
@@ -1,0 +1,14 @@
+module Libcrux_ecdh.P256_internal
+#set-options "--fuel 0 --ifuel 1 --z3rlimit 15"
+open FStar.Mul
+open Core_models
+
+type t_PrivateKey = | PrivateKey : t_Array u8 (mk_usize 32) -> t_PrivateKey
+
+type t_PublicKey = | PublicKey : t_Array u8 (mk_usize 64) -> t_PublicKey
+
+/// Output of a scalar multiplication between a public key and a secret key.
+/// This value is NOT (!) safe for use as a key and needs to be processed in a round of key
+/// derivation, to ensure both that the output is uniformly random and that unkown key share
+/// attacks can not happen.
+type t_SharedSecret = | SharedSecret : t_Array u8 (mk_usize 64) -> t_SharedSecret
