securedrop-protocol/protocol-minimal/proofs/fstar/models/Libcrux_ml_kem.Types.fsti
@@ -1,0 +1,13 @@
+module Libcrux_ml_kem.Types
+#set-options "--fuel 0 --ifuel 1 --z3rlimit 15"
+open FStar.Mul
+open Core_models
+
+///An ML-KEM Ciphertext
+type t_MlKemCiphertext (v_SIZE: usize) = { f_value:t_Array u8 v_SIZE }
+
+///An ML-KEM Private key
+type t_MlKemPrivateKey (v_SIZE: usize) = { f_value:t_Array u8 v_SIZE }
+
+///An ML-KEM Public key
+type t_MlKemPublicKey (v_SIZE: usize) = { f_value:t_Array u8 v_SIZE }
